completeness of the interpreter step function

examples/wysteria/interpreter.fst
@@ -1,7 +1,7 @@
 (*--build-config
-    options:--admit_fsi FStar.OrdSet --admit_fsi FStar.Seq --admit_fsi FStar.OrdMap --admit_fsi FStar.Set --admit_fsi Ffibridge --admit_fsi Runtime --admit_fsi FStar.IO --admit_fsi FStar.String --__temp_no_proj PSemantics --verify_module Interpreter;
+    options:--admit_fsi FStar.OrdSet --admit_fsi FStar.Seq --admit_fsi FStar.OrdMap --admit_fsi FStar.Set --admit_fsi Ffibridge --admit_fsi Runtime --admit_fsi FStar.IO --admit_fsi FStar.String --admit_fsi Hashtable --__temp_no_proj PSemantics --verify_module Interpreter;
     variables:CONTRIB=../../contrib;
-    other-files:classical.fst ext.fst set.fsi heap.fst st.fst all.fst seq.fsi seqproperties.fst ghost.fst listTot.fst ordset.fsi ordmap.fsi list.fst io.fsti string.fst prins.fst ast.fst ffibridge.fsi sem.fst psem.fst $CONTRIB/Platform/fst/Bytes.fst runtime.fsi print.fst ckt.fst $CONTRIB/CoreCrypto/fst/CoreCrypto.fst ../crypto/sha1.fst crypto.fst
+    other-files:classical.fst ext.fst set.fsi heap.fst st.fst all.fst seq.fsi seqproperties.fst ghost.fst listTot.fst ordset.fsi ordmap.fsi list.fst io.fsti string.fst prins.fst ast.fst ffibridge.fsi sem.fst psem.fst $CONTRIB/Platform/fst/Bytes.fst runtime.fsi print.fst hashtable.fsi ckt.fst $CONTRIB/CoreCrypto/fst/CoreCrypto.fst ../crypto/sha1.fst crypto.fst
  --*)
 
 module Interpreter
@@ -152,6 +152,9 @@ let step_correctness c =
   else if is_value c && is_sframe c is_F_assec_e then C_assec_red c c'
   else if not (pre_assec c = NA) then C_assec_beta c c'
   else C_assec_ret c c'
+
+val step_completeness: c:config -> c':config -> h:sstep c c' -> Lemma (requires (True)) (ensures (is_Some (step c)))
+let step_completeness c c' h = ()
 
 #set-options "--z3timeout 10"
 
